theories/case_studies/multiuser_kvs/kvs_main_spec.v
@@ -66,7 +66,8 @@ Section KVS_main_spec.
     (
       na_inv cerise_nais Nassert (assert_inv b_assert e_assert a_flag) ∗
       na_inv cerise_nais Nswitcher switcher_inv ∗
-      na_inv cerise_nais Nkvs kvs_inv ∗
+      na_inv cerise_nais (Nkvs.@"physical") kvs_inv ∗
+      na_inv cerise_nais (Nkvs.@"logical") logical_kvs_inv ∗
 
       inv (export_table_PCCN Nkvs_exp_tbl) (b_kvs_exp_tbl ↦ₐ WCap RX Global KVS_pcc_b KVS_pcc_e KVS_pcc_b) ∗
       inv (export_table_CGPN Nkvs_exp_tbl) ((b_kvs_exp_tbl ^+ 1)%a ↦ₐ WCap RW Global KVS_cgp_b KVS_cgp_e KVS_cgp_b) ∗
@@ -87,7 +88,7 @@ Section KVS_main_spec.
       [[ cgp_b , cgp_e ]] ↦ₐ [[ (kvs_main_data) ]] ∗
       [[ static_sealed_b , static_sealed_e ]] ↦ₐ [[ kvs_main_static_sealed KVS_USER_KEY_MAIN ]] ∗
 
-      logical_user_kvs_inv KVS_USER_KEY_MAIN ∗
+      user_kvs_inv KVS_USER_KEY_MAIN ∗
       (KVS_USER_KEY_MAIN, 1) ↦(KVS) ⊥ ∗
 
       world_interp W0 B ∗
@@ -105,7 +106,7 @@ Section KVS_main_spec.
                Hstatic_sealed_contiguous Hcgp_contiguous Himports_contiguous Hframe_match
             )
       "(#Hassert & #Hswitcher
-      & #Hkvs
+      & #Hkvs & #Hkvs_logical
       & #Hkvs_exp_tbl_pcc & #Hkvs_exp_tbl_cgp & #Hkvs_exp_tbl_addOrUpdate & #Hkvs_exp_tbl_read
       & Hna
       & HPC & Hcgp & Hcsp & Hrmap
@@ -316,7 +317,7 @@ Section KVS_main_spec.
 
     (* Use spec addOrUpdate known *)
     iApply (KVS_add_spec
-      with "[- $Hkvs $Hna $HPC $Hcgp $Hcra $ Hca0 $Hca1 $Hca2 $Hctp $Hct1 $Hct2 $Hcnull
+      with "[- $Hkvs $Hkvs_logical $Hna $HPC $Hcgp $Hcra $ Hca0 $Hca1 $Hca2 $Hctp $Hct1 $Hct2 $Hcnull
       $Hstatic_sealed_b $HLUKVS $Hkvs_1]")
     ; auto.
     { rewrite /is_uint16 /UINT16_MIN /UINT16_MAX; lia. }
@@ -648,7 +649,7 @@ Section KVS_main_spec.
 
     (* Use spec readOrUpdate known *)
     iApply (KVS_read_spec_in
-      with "[- $Hkvs $Hna $HPC $Hcgp $Hcra $Hca0 $Hca1 $Hct1 $Hct2 $Hctp $Hcnull
+      with "[- $Hkvs $Hkvs_logical $Hna $HPC $Hcgp $Hcra $Hca0 $Hca1 $Hct1 $Hct2 $Hctp $Hcnull
             $Hstatic_sealed_b $HLUKVS $Hkvs_1]")
     ; auto.
     { rewrite /is_uint16 /UINT16_MIN /UINT16_MAX; lia. }
