theories/case_studies/multiuser_kvs/kvs_spec_addOrUpdate.v
@@ -20,27 +20,27 @@ Section KVS_spec_addOrUpdate.
   .
 
   (*** KVS INSERT: Key in the KVS *)
-  Lemma KVS_update_spec_layer_1
-    (pc_b pc_e pc_a : Addr)
-    (cgp_b cgp_e : Addr)
+  Lemma KVS_update_spec_layer_0
     (wret wca2 : Word)
     (user_key : user_key_t) (nkey : map_key_t) (l_user_key : Locality) (user_key_addr : Addr)
-    (lkvs : kvs_logical_map) (m : kvs_user_map)
+    (idx : kvs_idx_t) ( wnkey : Word )
+    (pkvs : kvs_physical_map)
     :
 
     let fkey := (kvs_full_key user_key nkey) in
 
-    SubBounds pc_b pc_e pc_a (pc_a ^+ length kvs_addOrUpdate_instrs)%a ->
+    SubBounds KVS_pcc_b KVS_pcc_e kvs_addOrUpdate_pcc_addr (kvs_addOrUpdate_pcc_addr ^+ length kvs_addOrUpdate_instrs)%a ->
+    (KVS_cgp_b + length kvs_data)%a = Some KVS_cgp_e ->
+
     withinBounds user_key_addr (user_key_addr ^+ 1)%a user_key_addr = true ->
     is_uint16 nkey ->
 
-    (cgp_b + length kvs_data)%a = Some cgp_e ->
-
-    is_Some (m !! nkey) ->
+    pkvs !! idx = Some (Some (kvs_full_key user_key nkey, wnkey)) ->
 
     ((* initial register file *)
-      PC ↦ᵣ WCap RX Global pc_b pc_e pc_a ∗
-      cgp ↦ᵣ WCap RW Global cgp_b cgp_e cgp_b ∗
+
+      PC ↦ᵣ WCap RX Global KVS_pcc_b KVS_pcc_e kvs_addOrUpdate_pcc_addr ∗
+      cgp ↦ᵣ WCap RW Global KVS_cgp_b KVS_cgp_e KVS_cgp_b ∗
       cra ↦ᵣ wret ∗
       ca0 ↦ᵣ kvs_user_seal_key l_user_key user_key_addr ∗ (* Sealed User Key *)
       ca1 ↦ᵣ WInt nkey ∗ (* Key to update *)
@@ -51,13 +51,11 @@ Section KVS_spec_addOrUpdate.
       cnull ↦ᵣ - ∗
 
       (* initial memory layout *)
-      codefrag pc_a kvs_addOrUpdate_instrs ∗
-      (pc_b ^+ UNSEALING_USER_KEY_OFFSET)%a ↦ₐ kvs_service_unsealing_key ∗
+      codefrag kvs_addOrUpdate_pcc_addr kvs_addOrUpdate_instrs ∗
+      (KVS_pcc_b ^+ UNSEALING_USER_KEY_OFFSET)%a ↦ₐ kvs_service_unsealing_key ∗
       user_key_addr ↦ₐ WInt user_key ∗
 
-      ▷ ↪●LKVS lkvs ∗
-      ▷ is_logical_kvs cgp_b lkvs ∗
-      ▷ user_key ↦(LKVS) m ∗
+      ▷ is_physical_kvs KVS_cgp_b pkvs ∗
 
       ▷ (
           ⌜ canStore RW wca2 = true ⌝ ∗
@@ -72,24 +70,24 @@ Section KVS_spec_addOrUpdate.
           ct2 ↦ᵣ - ∗ (* scratch *)
           cnull ↦ᵣ - ∗
 
-          ↪●LKVS (<<[ (user_key, nkey):= wca2 ]>> lkvs) ∗
-          is_logical_kvs cgp_b (<<[ (user_key, nkey):= wca2 ]>> lkvs) ∗
-          user_key ↦(LKVS) (<[ nkey := wca2 ]> m) ∗
+          codefrag kvs_addOrUpdate_pcc_addr kvs_addOrUpdate_instrs ∗
+          (KVS_pcc_b ^+ UNSEALING_USER_KEY_OFFSET)%a ↦ₐ kvs_service_unsealing_key ∗
+          user_key_addr ↦ₐ WInt user_key ∗
 
-          codefrag pc_a kvs_addOrUpdate_instrs ∗
-          (pc_b ^+ UNSEALING_USER_KEY_OFFSET)%a ↦ₐ kvs_service_unsealing_key ∗
-          user_key_addr ↦ₐ WInt user_key
+          is_physical_kvs KVS_cgp_b (<[idx := Some (fkey, wca2)]> pkvs)
 
           -∗ WP Seq (Instr Executable) {{ v, ⌜v = HaltedV⌝ → na_own cerise_nais ⊤ }}
         )
       ⊢ WP Seq (Instr Executable) {{ v, ⌜v = HaltedV⌝ → na_own cerise_nais ⊤ }})%I.
   Proof.
     intros fkey.
-    iIntros (HsubBounds Hbounds_a_user_key His_uint16_nkey Hcgp_contiguous [wnkey Hm_nkey])
+    iIntros (Hbounds_pcc Hbounds_cgp Hbounds_a_user_key His_uint16_nkey Hpkvs_idx)
       "(HPC & Hcgp & Hcra & Hca0 & Hca1 & Hca2 & Hctp & Hct1 & Hct2 & [%wcnull Hcnull]
         & Hcode & Ha_unsealing & Ha_user_key
-        & Hlkvs_auth & (%pkvs & >%Hsync & HKVS) & Hm & Hpost)".
-    codefrag_facts "Hcode"; rename H into Hpc_contiguous ; clear H0.
+        & HPKVS & Hpost)".
+
+    codefrag_facts "Hcode"; rename H into Hpc_contiguous; clear H0.
+
 
     (* --------------------------------------------------- *)
     (* ----------------- Start the proof ----------------- *)
@@ -100,7 +98,7 @@ Section KVS_spec_addOrUpdate.
     rewrite -/(kvs_check_uint16 ca1 ct1).
 
     focus_block_0 "Hcode" as "Hcode" "Hcont"; iHide "Hcont" as hcont.
-    iApply (KVS_check_uint16_spec_is_uint16 with "[- $HPC $Hca1 $Hct1 $Hcode]"); eauto;iNext.
+    iApply (KVS_check_uint16_spec_is_uint16 with "[- $HPC $Hca1 $Hct1 $Hcode]"); eauto; iNext.
     iIntros "(HPC & Hca1 & Hcode & Hct1)".
     subst hcont; unfocus_block "Hcode" "Hcont" as "Hcode".
 
@@ -121,16 +119,11 @@ Section KVS_spec_addOrUpdate.
     iInstr "Hcode".
     subst hcont; unfocus_block "Hcode" "Hcont" as "Hcode".
 
-    iDestruct ( kvs_logical_kvs_valid with "Hlkvs_auth Hm" ) as "%Hlkvs_user_key".
-    pose proof (kvs_synced_logical_lookup_Some _ _ _ _ _ _
-                  His_uint16_nkey Hsync Hlkvs_user_key Hm_nkey)
-      as (idx & Hpkvs_idx).
-
     focus_block 4 "Hcode" as a_search Ha_search "Hcode" "Hcont"; iHide "Hcont" as hcont; clear dependent Ha_lea.
-    iApply (KVS_search_spec_in with "[- $HPC $Hcgp $Hca0 $Hctp $Hct1 $Hct2 $HKVS $Hcode]"); eauto.
+    iApply (KVS_search_spec_in with "[- $HPC $Hcgp $Hca0 $Hctp $Hct1 $Hct2 $HPKVS $Hcode]"); eauto.
     { rewrite /withinBounds; solve_addr. }
     iNext; iIntros "(HPC & Hcgp & Hca0 & Hctp & Hct1 & Hct2 & Hcgp_opt & Hcgp_key & Hcgp_val
-                    & HKVS & %Hcgp_idx & Hcode)".
+                    & HPKVS & %Hcgp_idx & Hcode)".
     subst hcont; unfocus_block "Hcode" "Hcont" as "Hcode".
 
     focus_block 5 "Hcode" as a_addOrUpdate Ha_addOrUpdate "Hcode" "Hcont"; iHide "Hcont" as hcont; clear dependent Ha_search.
@@ -141,7 +134,7 @@ Section KVS_spec_addOrUpdate.
     { injection; intros; lia. }
     (* Lea cgp 2 *)
     iInstr "Hcode".
-    { transitivity ( Some ((cgp_b ^+ (ASM_SIZEOF_KVS_ENTRY * idx + 2))%a) ); last done; solve_addr+Hcgp_idx. }
+    { transitivity ( Some ((KVS_cgp_b ^+ (ASM_SIZEOF_KVS_ENTRY * idx + 2))%a) ); last done; solve_addr+Hcgp_idx. }
     (* Store cgp (inr ca2) *)
     destruct (canStore RW wca2) eqn:HcanStore_wca2; cycle 1.
     {
@@ -166,17 +159,144 @@ Section KVS_spec_addOrUpdate.
     iInstr "Hcode".
     subst hcont; unfocus_block "Hcode" "Hcont" as "Hcode".
 
-    iDestruct (is_physical_kvs_open_wf with "HKVS") as "[%_ %Hnodup_pkvs_keys]".
-    iDestruct (kvs_physical_map_close_update with "[$HKVS] [Hcgp_opt Hcgp_key Hcgp_val]")
-      as "HKVS"; eauto.
+    iDestruct (is_physical_kvs_open_wf with "HPKVS") as "[%_ %Hnodup_pkvs_keys]".
+    iDestruct (kvs_physical_map_close_update with "[$HPKVS] [Hcgp_opt Hcgp_key Hcgp_val]")
+      as "HPKVS"; eauto.
     { iApply destruct_physical_kvs_entry; first solve_addr; iFrame. }
 
+    iApply "Hpost"; iFrame "∗%"; done.
+  Qed.
+
+  Lemma KVS_update_spec_layer_1
+    (wret wca2 : Word)
+    (user_key : user_key_t) (nkey : map_key_t) (l_user_key : Locality) (user_key_addr : Addr)
+    (lkvs : kvs_logical_map) (m : kvs_user_map)
+    (E : coPset)
+    :
+
+    let fkey := (kvs_full_key user_key nkey) in
+
+    ↑(Nkvs.@"physical") ⊆ E ->
+
+    withinBounds user_key_addr (user_key_addr ^+ 1)%a user_key_addr = true ->
+    is_uint16 nkey ->
+
+    is_Some (m !! nkey) ->
+
+    ( na_inv cerise_nais (Nkvs.@"physical") kvs_inv ∗
+      na_own cerise_nais E ∗
+
+      (* initial register file *)
+
+      PC ↦ᵣ WCap RX Global KVS_pcc_b KVS_pcc_e kvs_addOrUpdate_pcc_addr ∗
+      cgp ↦ᵣ WCap RW Global KVS_cgp_b KVS_cgp_e KVS_cgp_b ∗
+      cra ↦ᵣ wret ∗
+      ca0 ↦ᵣ kvs_user_seal_key l_user_key user_key_addr ∗ (* Sealed User Key *)
+      ca1 ↦ᵣ WInt nkey ∗ (* Key to update *)
+      ca2 ↦ᵣ wca2 ∗ (* New value *)
+      ctp ↦ᵣ - ∗ (* scratch *)
+      ct1 ↦ᵣ - ∗ (* scratch *)
+      ct2 ↦ᵣ - ∗ (* scratch *)
+      cnull ↦ᵣ - ∗
+
+      (* initial memory layout *)
+      user_key_addr ↦ₐ WInt user_key ∗
+
+      ▷ ↪●LKVS lkvs ∗
+      ▷ is_logical_kvs lkvs ∗
+      ▷ user_key ↦(LKVS) m ∗
+
+      ▷ (
+          ⌜ canStore RW wca2 = true ⌝ ∗
+          na_own cerise_nais E ∗
+
+          PC ↦ᵣ updatePcPerm wret ∗
+          cgp ↦ᵣ - ∗
+          cra ↦ᵣ - ∗
+          ca0 ↦ᵣ WInt ASM_TRUE ∗ (* TRUE: the key exists in the map and is updated *)
+          ca1 ↦ᵣ WInt 0 ∗
+          ca2 ↦ᵣ - ∗
+          ctp ↦ᵣ - ∗ (* scratch *)
+          ct1 ↦ᵣ - ∗ (* scratch *)
+          ct2 ↦ᵣ - ∗ (* scratch *)
+          cnull ↦ᵣ - ∗
+
+          user_key_addr ↦ₐ WInt user_key ∗
+
+          ↪●LKVS (<<[ (user_key, nkey):= wca2 ]>> lkvs) ∗
+          is_logical_kvs (<<[ (user_key, nkey):= wca2 ]>> lkvs) ∗
+          user_key ↦(LKVS) (<[ nkey := wca2 ]> m)
+
+          -∗ WP Seq (Instr Executable) {{ v, ⌜v = HaltedV⌝ → na_own cerise_nais ⊤ }}
+        )
+      ⊢ WP Seq (Instr Executable) {{ v, ⌜v = HaltedV⌝ → na_own cerise_nais ⊤ }})%I.
+  Proof.
+    intros fkey.
+    iIntros (Hnkvs_E Hbounds_a_user_key His_uint16_nkey [wnkey Hm_nkey])
+      "(#Hkvs_inv & Hna
+        & HPC & Hcgp & Hcra & Hca0 & Hca1 & Hca2 & Hctp & Hct1 & Hct2 & Hcnull
+        & Ha_user_key
+        & >Hlkvs_auth & (%pkvs & >%Hsync & >Hpkvs_frag) & >Hm & Hpost)".
+    iMod (na_inv_acc with "Hkvs_inv Hna")
+      as "( (>Himports & >Hcode & (%pkvs' & HPKVS & >Hpkvs_frag')) & Hna & Hkvs_inv_close)"; eauto.
+
+    pose proof (HKVS_pcc_b' := KVS_size_imports).
+    pose proof (Hcode_continuous := KVS_size_code).
+    pose proof (Hcgp_continuous := KVS_size_data).
+    assert ((KVS_cgp_b + length kvs_data)%a = Some KVS_cgp_e) as Hbounds_cgp.
+    { by rewrite /length_kvs_data in Hcgp_continuous. }
+
+    rewrite /kvs_imports /kvs.kvs_imports_pre.
+    assert ((KVS_pcc_b + 1)%a = Some (KVS_pcc_b ^+ 1)%a) by ( rewrite /length_kvs_imports in HKVS_pcc_b'; solve_addr+ HKVS_pcc_b').
+    assert ((KVS_pcc_b ^+ 1)%a <= KVS_pcc_b')%a  by ( rewrite /length_kvs_imports in HKVS_pcc_b'; solve_addr+ HKVS_pcc_b').
+    assert ((KVS_pcc_b ^+ 1 + 1)%a = Some (KVS_pcc_b')%a) by ( rewrite /length_kvs_imports in HKVS_pcc_b'; solve_addr+ HKVS_pcc_b').
+    iDestruct (region_pointsto_cons with "Himports") as "[Himports_sw Himports]"; eauto.
+    iDestruct (region_pointsto_single with "Himports") as "(% & Ha_unsealing & %Heq)"; eauto; simplify_eq.
+    assert (SubBounds KVS_pcc_b KVS_pcc_e KVS_pcc_b' (KVS_pcc_b' ^+ length kvs_service_instrs)%a) as HSubBounds.
+    { solve_addr. }
+
+    focus_block_0 "Hcode" as "Hcode" "Hcont"; iHide "Hcont" as hcont.
+    assert (kvs_addOrUpdate_pcc_addr = KVS_pcc_b') as Heq_addr
+       by (rewrite /kvs_addOrUpdate_pcc_addr /kvs_addOrUpdate_pcc_off; solve_addr+HKVS_pcc_b').
+    rewrite -Heq_addr in H3; rewrite -Heq_addr.
+
+    iDestruct ( kvs_physical_kvs_valid with "Hpkvs_frag Hpkvs_frag'") as "<-".
+
+    iDestruct ( kvs_logical_kvs_valid with "Hlkvs_auth Hm" ) as "%Hlkvs_user_key".
+    pose proof (kvs_synced_logical_lookup_Some _ _ _ _ _ _
+                  His_uint16_nkey Hsync Hlkvs_user_key Hm_nkey)
+      as (idx & Hpkvs_idx).
+
+    iDestruct (is_physical_kvs_wf with "HPKVS") as "#[_ Hnodup_pkvs]".
+
+
+    iApply (KVS_update_spec_layer_0 with
+             "[- $HPC $Hcgp $Hcra $Hca0 $Hca1 $Hca2 $Hctp $Hct1 $Hct2 $Hcnull
+              $Hcode $Ha_unsealing $Ha_user_key
+              $HPKVS]"); eauto.
+    iNext; iIntros "(%Hcan_store & HPC & Hcgp & Hcra & Hca0 & Hca1 & Hca2 & Hctp & Hct1 & Hct2 & Hcnull
+                     & Hcode & Ha_unsealing & Ha_user_key
+                     & HPKVS )".
+    rewrite Heq_addr.
+    subst hcont; unfocus_block "Hcode" "Hcont" as "Hcode".
+
+    iMod (kvs_physical_kvs_update (<[idx:=Some (kvs_full_key user_key nkey, wca2)]> pkvs) with
+           "Hpkvs_frag Hpkvs_frag'") as "[Hpkvs_frag Hpkvs_frag']".
+
+    iMod ("Hkvs_inv_close" with "[$Hna $Hcode Himports_sw Ha_unsealing $HPKVS $Hpkvs_frag']") as "Hna" ; auto.
+    { iNext.
+      iApply (region_pointsto_cons with "[Ha_unsealing Himports_sw]"); eauto; iFrame.
+      iApply (region_pointsto_cons with "[Ha_unsealing]"); eauto; [solve_addr+|]; iFrame.
+      rewrite /region_pointsto finz_seq_between_empty; auto; solve_addr+.
+    }
+
+    iDestruct "Hnodup_pkvs" as "%Hnodup_pkvs".
     iMod ( kvs_logical_kvs_update user_key _ _ (<[nkey := wca2]> m) with "Hlkvs_auth Hm" ) as "[Hlkvs_auth Hm]".
     replace ( <[user_key:=<[nkey:=wca2]> m]> lkvs ) with ( <<[ (user_key, nkey):= wca2 ]>> lkvs ).
     2: { rewrite /kvs_logical_kvs_insert Hlkvs_user_key //. }
     eapply (kvs_synced_logical_kvs_update _ _ _ _ _ wca2) in Hsync; eauto.
 
-    iApply "Hpost"; iFrame "∗%"; done.
+    iApply "Hpost"; iFrame; done.
   Qed.
 
   Lemma KVS_update_spec_layer_2
@@ -187,14 +307,16 @@ Section KVS_spec_addOrUpdate.
     :
     let fkey := (kvs_full_key user_key nkey) in
 
-    ↑Nkvs ⊆ E ->
+    ↑(Nkvs.@"physical") ⊆ E ->
+    ↑(Nkvs.@"logical") ⊆ E ->
 
     is_uint16 nkey ->
     withinBounds user_key_addr (user_key_addr ^+ 1)%a user_key_addr = true ->
 
     is_Some (m !! nkey) ->
 
-    ( na_inv cerise_nais Nkvs kvs_inv ∗
+    ( na_inv cerise_nais (Nkvs.@"physical") kvs_inv ∗
+      na_inv cerise_nais (Nkvs.@"logical") logical_kvs_inv ∗
       na_own cerise_nais E ∗
 
       (* initial register file *)
@@ -234,39 +356,26 @@ Section KVS_spec_addOrUpdate.
       ⊢ WP Seq (Instr Executable) {{ v, ⌜v = HaltedV⌝ → na_own cerise_nais ⊤ }})%I.
   Proof.
     intros fkey.
-    iIntros (Hnkvs_E His_uint16_nkey Hbounds_a_user_key Hm_nkey)
-      "(#Hkvs_inv & Hna & HPC & Hcgp & Hcra & Hca0 & Hca1 & Hca2 & Hctp & Hct1 & Hct2 & Hcnull
+    iIntros (Hnkvs_E Hnkvs_E' His_uint16_nkey Hbounds_a_user_key Hm_nkey)
+      "(#Hkvs_inv & #Hkvs_logical_inv & Hna
+      & HPC & Hcgp & Hcra & Hca0 & Hca1 & Hca2 & Hctp & Hct1 & Hct2 & Hcnull
       & Ha_user_key & Hm & Hpost)".
-    iMod (na_inv_acc with "Hkvs_inv Hna")
-      as "( (>Himports & >Hcode & (%lkvs & Hlkvs_auth & HKVS) & Hspred) & Hna & Hkvs_inv_close)"; eauto.
-    pose proof (Hcgp_continuous := KVS_size_data).
-    pose proof (HKVS_pcc_b' := KVS_size_imports).
-    pose proof (Hcode_continuous := KVS_size_code).
-    assert (SubBounds KVS_pcc_b KVS_pcc_e KVS_pcc_b' (KVS_pcc_b' ^+ length kvs_service_instrs)%a) as HSubBounds.
-    { solve_addr. }
-    codefrag_facts "Hcode"; rename H into Hpc_contiguous.
-    rewrite /kvs_imports /kvs.kvs_imports_pre.
-    assert ((KVS_pcc_b + 1)%a = Some (KVS_pcc_b ^+ 1)%a) by ( rewrite /length_kvs_imports in HKVS_pcc_b'; solve_addr+ HKVS_pcc_b').
-    assert ((KVS_pcc_b ^+ 1)%a <= KVS_pcc_b')%a  by ( rewrite /length_kvs_imports in HKVS_pcc_b'; solve_addr+ HKVS_pcc_b').
-    assert ((KVS_pcc_b ^+ 1 + 1)%a = Some (KVS_pcc_b')%a) by ( rewrite /length_kvs_imports in HKVS_pcc_b'; solve_addr+ HKVS_pcc_b').
-    iDestruct (region_pointsto_cons with "Himports") as "[Himports_sw Himports]"; eauto.
-    iDestruct (region_pointsto_single with "Himports") as "(% & Ha_unsealing & %Heq)"; eauto; simplify_eq.
+    iMod (na_inv_acc with "Hkvs_logical_inv Hna")
+      as "( (%lkvs & Hlkvs_auth & HLKVS) & Hna & Hkvs_logical_inv_close)"; eauto.
 
-    rewrite /kvs_service_instrs.
-    focus_block_0 "Hcode" as "Hcode" "Hcont"; iHide "Hcont" as hcont.
-    assert (kvs_addOrUpdate_pcc_addr = KVS_pcc_b')
-      as -> by (rewrite /kvs_addOrUpdate_pcc_addr /kvs_addOrUpdate_pcc_off; solve_addr+HKVS_pcc_b').
-    iApply (KVS_update_spec_layer_1 with "[- $HPC]"); last iFrame; eauto.
-    iNext; iIntros "(%Hcan_store & HPC & Hcgp & Hcra & Hca0 & Hca1 & Hca2 & Hctp & Hct1 & Hct2
-              & Hcnull & Hlkvs_auth & HKVS & Hm & Hcode & Ha_unsealing & Ha_user_key)".
-    subst hcont; unfocus_block "Hcode" "Hcont" as "Hcode".
+    iApply (KVS_update_spec_layer_1 with
+             "[- $Hkvs_inv
+                 $HPC $Hcgp $Hcra $Hca0 $Hca1 $Hca2 $Hctp $Hct1 $Hct2 $Hcnull
+                 $Ha_user_key
+                 $Hlkvs_auth $HLKVS $Hm]"); last iFrame; eauto.
+    {  solve_ndisj. }
 
-    iMod ("Hkvs_inv_close" with "[$Hna $Hcode Himports_sw Ha_unsealing $Hlkvs_auth $HKVS $Hspred]") as "Hna" ; auto.
-    { iNext.
-      iApply (region_pointsto_cons with "[Ha_unsealing Himports_sw]"); eauto; iFrame.
-      iApply (region_pointsto_cons with "[Ha_unsealing]"); eauto; [solve_addr+|]; iFrame.
-      rewrite /region_pointsto finz_seq_between_empty; auto; solve_addr+.
-    }
+    iNext; iIntros "(%Hcan_store & Hna
+                     & HPC & Hcgp & Hcra & Hca0 & Hca1 & Hca2 & Hctp & Hct1 & Hct2 & Hcnull
+                     & Ha_user_key
+                     & Hlkvs_auth & HLKVS & Hm)".
+
+    iMod ("Hkvs_logical_inv_close" with "[$Hna $Hlkvs_auth $HLKVS]") as "Hna" ; auto.
     iApply "Hpost"; iFrame; done.
   Qed.
 
@@ -278,12 +387,14 @@ Section KVS_spec_addOrUpdate.
     :
     let fkey := (kvs_full_key user_key nkey) in
 
-    ↑Nkvs ⊆ E ->
+    ↑(Nkvs.@"physical") ⊆ E ->
+    ↑(Nkvs.@"logical") ⊆ E ->
 
     is_uint16 nkey ->
     withinBounds user_key_addr (user_key_addr ^+ 1)%a user_key_addr = true ->
 
-    ( na_inv cerise_nais Nkvs kvs_inv ∗
+    ( na_inv cerise_nais (Nkvs.@"physical") kvs_inv ∗
+      na_inv cerise_nais (Nkvs.@"logical") logical_kvs_inv ∗
       na_own cerise_nais E ∗
 
       (* initial register file *)
@@ -300,7 +411,7 @@ Section KVS_spec_addOrUpdate.
 
       user_key_addr ↦ₐ WInt user_key ∗
 
-      ▷ logical_user_kvs_inv user_key ∗
+      ▷ user_kvs_inv user_key ∗
       ▷ (user_key, nkey) ↦(KVS) - ∗
 
       ▷ ( ⌜ canStore RW wca2 = true ⌝ ∗
@@ -317,7 +428,7 @@ Section KVS_spec_addOrUpdate.
           cnull ↦ᵣ - ∗
           user_key_addr ↦ₐ WInt user_key ∗
 
-          logical_user_kvs_inv user_key ∗
+          user_kvs_inv user_key ∗
           (user_key, nkey) ↦(KVS) wca2
 
          -∗ WP Seq (Instr Executable) {{ v, ⌜v = HaltedV⌝ → na_own cerise_nais ⊤ }}
@@ -325,51 +436,51 @@ Section KVS_spec_addOrUpdate.
       ⊢ WP Seq (Instr Executable) {{ v, ⌜v = HaltedV⌝ → na_own cerise_nais ⊤ }})%I.
   Proof.
     intros fkey.
-    iIntros (Hnkvs_E His_uint16_nkey Hbounds_a_user_key)
-      "(#Hkvs_inv & Hna & HPC & Hcgp & Hcra & Hca0 & Hca1 & Hca2 & Hctp & Hct1 & Hct2 & Hcnull
+    iIntros (Hnkvs_E Hnkvs_E' His_uint16_nkey Hbounds_a_user_key)
+      "(#Hkvs_inv & #Hkvs_logical_inv & Hna
+      & HPC & Hcgp & Hcra & Hca0 & Hca1 & Hca2 & Hctp & Hct1 & Hct2 & Hcnull
       & Ha_user_key & (%ukvs & >Hukvs_auth & (%m & Hm & >%Hsync)) & [%wk >Hk] & Hpost)".
 
     iDestruct (kvs_user_kvs_valid with "Hukvs_auth Hk") as "%Hk".
     opose proof (kvs_synced_logical_user_kvs_Some _ _ _ _ _ Hk) as Hm_kvs; eauto.
 
     iApply (KVS_update_spec_layer_2
-             with "[- $Hkvs_inv $Hna
+             with "[- $Hkvs_inv $Hkvs_logical_inv $Hna
                     $HPC $Hcgp $Hcra $Hca0 $Hca1 $Hca2 $Hctp $Hct1 $Hct2 $Hcnull
-                    $Ha_user_key $Hm]"); eauto.
+                    $Ha_user_key
+                    $Hm]"); eauto.
     iNext; iIntros "(%Hcan_store & Hna
                      & HPC & Hcgp & Hcra & Hca0 & Hca1 & Hca2 & Hctp & Hct1 & Hct2 & Hcnull
-                     & Ha_user_key & Hm)".
+                     & Ha_user_key
+                     & Hm)".
 
     iMod ( kvs_user_kvs_update _ _ _ _ (Some wca2) with "Hukvs_auth Hk" ) as "[Hukvs_auth Hk]".
     apply (kvs_synced_logical_user_kvs_insert _ _ nkey wca2) in Hsync.
-    iAssert (logical_user_kvs_inv user_key)%I with "[$Hm $Hukvs_auth]" as "Hlukvs"; auto.
+    iAssert (user_kvs_inv user_key)%I with "[$Hm $Hukvs_auth]" as "Hlukvs"; auto.
 
     iApply "Hpost"; iFrame; done.
   Qed.
 
-  (*** KVS INSERT: Key not in the KVS *)
-  Lemma KVS_add_spec_layer_1
-    (pc_b pc_e pc_a : Addr)
-    (cgp_b cgp_e : Addr)
+  Lemma KVS_add_spec_layer_0
     (wret wca2 : Word)
     (user_key : user_key_t) (nkey : map_key_t) (l_user_key : Locality) (user_key_addr : Addr)
-    (lkvs : kvs_logical_map) (m : kvs_user_map)
+    (pkvs : kvs_physical_map)
     :
 
     let fkey := (kvs_full_key user_key nkey) in
 
-    SubBounds pc_b pc_e pc_a (pc_a ^+ length kvs_addOrUpdate_instrs)%a ->
+    SubBounds KVS_pcc_b KVS_pcc_e kvs_addOrUpdate_pcc_addr (kvs_addOrUpdate_pcc_addr ^+ length kvs_addOrUpdate_instrs)%a ->
+    (KVS_cgp_b + length kvs_data)%a = Some KVS_cgp_e ->
+
     withinBounds user_key_addr (user_key_addr ^+ 1)%a user_key_addr = true ->
     is_uint16 nkey ->
 
-    (cgp_b + length kvs_data)%a = Some cgp_e ->
+    fkey ∉ kvs_keys pkvs ->
 
-    m !! nkey = None ->
+    ((* initial register file *)
 
-    (
-      (* initial register file *)
-      PC ↦ᵣ WCap RX Global pc_b pc_e pc_a ∗
-      cgp ↦ᵣ WCap RW Global cgp_b cgp_e cgp_b ∗
+      PC ↦ᵣ WCap RX Global KVS_pcc_b KVS_pcc_e kvs_addOrUpdate_pcc_addr ∗
+      cgp ↦ᵣ WCap RW Global KVS_cgp_b KVS_cgp_e KVS_cgp_b ∗
       cra ↦ᵣ wret ∗
       ca0 ↦ᵣ kvs_user_seal_key l_user_key user_key_addr ∗ (* Sealed User Key *)
       ca1 ↦ᵣ WInt nkey ∗ (* Key to update *)
@@ -380,15 +491,14 @@ Section KVS_spec_addOrUpdate.
       cnull ↦ᵣ - ∗
 
       (* initial memory layout *)
-      codefrag pc_a kvs_addOrUpdate_instrs ∗
-      (pc_b ^+ UNSEALING_USER_KEY_OFFSET)%a ↦ₐ kvs_service_unsealing_key ∗
+      codefrag kvs_addOrUpdate_pcc_addr kvs_addOrUpdate_instrs ∗
+      (KVS_pcc_b ^+ UNSEALING_USER_KEY_OFFSET)%a ↦ₐ kvs_service_unsealing_key ∗
       user_key_addr ↦ₐ WInt user_key ∗
 
-      ▷ ↪●LKVS lkvs ∗
-      ▷ is_logical_kvs cgp_b lkvs ∗
-      ▷ user_key ↦(LKVS) m ∗
+      ▷ is_physical_kvs KVS_cgp_b pkvs ∗
 
-      ▷ (PC ↦ᵣ updatePcPerm wret ∗
+      ▷ (
+          PC ↦ᵣ updatePcPerm wret ∗
           cgp ↦ᵣ - ∗
           cra ↦ᵣ - ∗
           ca1 ↦ᵣ WInt 0 ∗
@@ -397,38 +507,41 @@ Section KVS_spec_addOrUpdate.
           ct1 ↦ᵣ - ∗ (* scratch *)
           ct2 ↦ᵣ - ∗ (* scratch *)
           cnull ↦ᵣ - ∗
-          codefrag pc_a kvs_addOrUpdate_instrs ∗
-          (pc_b ^+ UNSEALING_USER_KEY_OFFSET)%a ↦ₐ kvs_service_unsealing_key ∗
+
+          codefrag kvs_addOrUpdate_pcc_addr kvs_addOrUpdate_instrs ∗
+          (KVS_pcc_b ^+ UNSEALING_USER_KEY_OFFSET)%a ↦ₐ kvs_service_unsealing_key ∗
           user_key_addr ↦ₐ WInt user_key ∗
+
           (
             (* THERE IS AN EMPTY SLOT AVAILABLE*)
-            ( ⌜ canStore RW wca2 = true ⌝ ∗
+            ( ∃ idx_empty,
+
+              ⌜ pkvs !! idx_empty = Some None ⌝ ∗
+              ⌜ canStore RW wca2 = true ⌝ ∗
               ca0 ↦ᵣ WInt ASM_TRUE ∗ (* TRUE: an empty slot is available and is updated *)
 
-              ↪●LKVS (<<[ ( user_key, nkey ) := wca2 ]>> lkvs) ∗
-              is_logical_kvs cgp_b (<<[ ( user_key, nkey ) := wca2 ]>> lkvs) ∗
-              user_key ↦(LKVS) (<[ nkey := wca2 ]> m)
+              is_physical_kvs KVS_cgp_b (<[idx_empty := Some (fkey, wca2)]> pkvs)
             )
             ∨
               (* THERE IS NO EMPTY SLOT AVAILABLE*)
               (
                 ca0 ↦ᵣ WInt ASM_FALSE ∗ (* FALSE: no empty slot available *)
-                ↪●LKVS lkvs ∗
-                is_logical_kvs cgp_b lkvs ∗
-                user_key ↦(LKVS) m
+                is_physical_kvs KVS_cgp_b pkvs
               )
           )
-          -∗
-          WP Seq (Instr Executable) {{ v, ⌜v = HaltedV⌝ → na_own cerise_nais ⊤ }}
+           -∗
+           WP Seq (Instr Executable) {{ v, ⌜v = HaltedV⌝ → na_own cerise_nais ⊤ }}
         )
       ⊢ WP Seq (Instr Executable) {{ v, ⌜v = HaltedV⌝ → na_own cerise_nais ⊤ }})%I.
   Proof.
     intros fkey.
-    iIntros (HsubBounds Hbounds_a_user_key His_uint16_nkey Hcgp_contiguous Hm_nkey)
-      "(HPC & Hcgp & Hcra & Hca0 & Hca1 & Hca2 & [%wctp Hctp] & Hct1 & Hct2 & [%wcnull Hcnull]
+    iIntros (Hbounds_pcc Hbounds_cgp Hbounds_a_user_key His_uint16_nkey Hpkvs_idx)
+      "(HPC & Hcgp & Hcra & Hca0 & Hca1 & Hca2 & Hctp & Hct1 & Hct2 & [%wcnull Hcnull]
         & Hcode & Ha_unsealing & Ha_user_key
-        & Hlkvs_auth & (%pkvs & >%Hsync & HKVS) & Hm & Hpost)".
-    codefrag_facts "Hcode"; rename H into Hpc_contiguous ; clear H0.
+        & HPKVS & Hpost)".
+
+    codefrag_facts "Hcode"; rename H into Hpc_contiguous; clear H0.
+
 
     (* --------------------------------------------------- *)
     (* ----------------- Start the proof ----------------- *)
@@ -436,9 +549,10 @@ Section KVS_spec_addOrUpdate.
     rewrite /kvs_addOrUpdate_instrs /assembled_kvs_addOrUpdate.
     rewrite -/(kvs_getFullKey ctp ca0 ca1 ct1 ct2).
     rewrite -/(kvs_search ca0 ctp ct1 ct2).
+    rewrite -/(kvs_check_uint16 ca1 ct1).
 
     focus_block_0 "Hcode" as "Hcode" "Hcont"; iHide "Hcont" as hcont.
-    iApply (KVS_check_uint16_spec_is_uint16 with "[- $HPC $Hca1 $Hct1 $Hcode]"); eauto;iNext.
+    iApply (KVS_check_uint16_spec_is_uint16 with "[- $HPC $Hca1 $Hct1 $Hcode]"); eauto; iNext.
     iIntros "(HPC & Hca1 & Hcode & Hct1)".
     subst hcont; unfocus_block "Hcode" "Hcont" as "Hcode".
 
@@ -459,19 +573,14 @@ Section KVS_spec_addOrUpdate.
     iInstr "Hcode".
     subst hcont; unfocus_block "Hcode" "Hcont" as "Hcode".
 
-    iDestruct ( kvs_logical_kvs_valid with "Hlkvs_auth Hm" ) as "%Hlkvs_user_key".
-    pose proof (kvs_synced_logical_lookup_None _ _ _ _ _
-                  His_uint16_nkey Hsync Hlkvs_user_key Hm_nkey)
-      as Hpkvs_idx.
-
     focus_block 4 "Hcode" as a_search Ha_search "Hcode" "Hcont"; iHide "Hcont" as hcont; clear dependent Ha_lea.
-    iApply (KVS_search_spec_empty_slot with "[- $HPC $Hcgp $Hca0 $Hctp $Hct1 $Hct2 $HKVS $Hcode]"); eauto.
+    iApply (KVS_search_spec_empty_slot with "[- $HPC $Hcgp $Hca0 $Hctp $Hct1 $Hct2 $HPKVS $Hcode]"); eauto.
     { rewrite /withinBounds; solve_addr. }
     iNext; iIntros "[
-    (%idx_empty & HPC & Hcgp & Hca0 & Hctp & Hct1 & Hct2 & HKVS
+    (%idx_empty & HPC & Hcgp & Hca0 & Hctp & Hct1 & Hct2 & HPKVS
     & Hcgp_opt & [%wkey Hcgp_key] & [%wval Hcgp_val] & %Hcgp_bounds
     & %Hidx_empty & %Hpkvs_idx_empty & Hcode)
-    | (HPC & Hcgp & Hca0 & Hctp & Hct1 & Hct2 & HKVS & Hcode) ]".
+    | (HPC & Hcgp & Hca0 & Hctp & Hct1 & Hct2 & HPKVS & Hcode) ]".
     all: subst hcont; unfocus_block "Hcode" "Hcont" as "Hcode".
 
     - (* An empty slot was found *)
@@ -490,13 +599,13 @@ Section KVS_spec_addOrUpdate.
       iInstr "Hcode".
       (* lea cgp ct1; *)
       iInstr "Hcode".
-      { transitivity (Some (cgp_b ^+ ASM_SIZEOF_KVS_ENTRY * idx_empty)%a); solve_addr+ Hidx_empty Hcgp_bounds. }
+      { transitivity (Some (KVS_cgp_b ^+ ASM_SIZEOF_KVS_ENTRY * idx_empty)%a); solve_addr+ Hidx_empty Hcgp_bounds. }
       (* store cgp ASM_SOME; *)
       iInstr "Hcode".
       { solve_addr+Hcgp_bounds. }
       (* lea cgp 1; *)
       iInstr "Hcode".
-      { transitivity (Some (cgp_b ^+ (ASM_SIZEOF_KVS_ENTRY * idx_empty + 1))%a); solve_addr+ Hidx_empty Hcgp_bounds. }
+      { transitivity (Some (KVS_cgp_b ^+ (ASM_SIZEOF_KVS_ENTRY * idx_empty + 1))%a); solve_addr+ Hidx_empty Hcgp_bounds. }
       (* store cgp ca0; *)
       iInstr_lookup "Hcode" as "Hi" "Hcode".
       wp_instr.
@@ -508,7 +617,7 @@ Section KVS_spec_addOrUpdate.
       iInstr_close "Hcode".
       (* lea cgp 1; *)
       iInstr "Hcode".
-      { transitivity (Some (cgp_b ^+ (ASM_SIZEOF_KVS_ENTRY * idx_empty + 2))%a); solve_addr+ Hidx_empty Hcgp_bounds. }
+      { transitivity (Some (KVS_cgp_b ^+ (ASM_SIZEOF_KVS_ENTRY * idx_empty + 2))%a); solve_addr+ Hidx_empty Hcgp_bounds. }
       (* store cgp ca2; *)
       destruct (canStore RW wca2) eqn:HcanStore_wca2; cycle 1.
       {
@@ -532,19 +641,15 @@ Section KVS_spec_addOrUpdate.
       iInstr "Hcode".
       subst hcont; unfocus_block "Hcode" "Hcont" as "Hcode".
 
-      iDestruct (is_physical_kvs_open_wf with "HKVS") as "[%_ %Hnodup_pkvs_keys]".
-      iDestruct (kvs_physical_map_close_insert with "[$HKVS] [Hcgp_opt Hcgp_key Hcgp_val]")
-        as "HKVS"; eauto.
+      iDestruct (is_physical_kvs_open_wf with "HPKVS") as "[%_ %Hnodup_pkvs_keys]".
+      iDestruct (kvs_physical_map_close_insert with "[$HPKVS] [Hcgp_opt Hcgp_key Hcgp_val]")
+        as "HPKVS"; eauto.
       { iApply destruct_physical_kvs_entry; first solve_addr; iFrame. }
-
-      iMod ( kvs_logical_kvs_update user_key _ _ (<[nkey := wca2]> m) with "Hlkvs_auth Hm" ) as "[Hlkvs_auth Hm]".
-      replace ( <[user_key:=<[nkey:=wca2]> m]> lkvs ) with ( <<[ (user_key, nkey):= wca2 ]>> lkvs ).
-      2: { rewrite /kvs_logical_kvs_insert Hlkvs_user_key //. }
-      eapply (kvs_synced_logical_kvs_insert _ _ _ _ _ wca2) in Hsync; eauto.
 
 
       iApply "Hpost"; iFrame "∗%".
       iLeft ; iFrame; done.
+
 
     - (* No empty slot found *)
 
@@ -572,6 +677,158 @@ Section KVS_spec_addOrUpdate.
       iRight ; iFrame.
   Qed.
 
+
+  (*** KVS INSERT: Key not in the KVS *)
+  Lemma KVS_add_spec_layer_1
+    (wret wca2 : Word)
+    (user_key : user_key_t) (nkey : map_key_t) (l_user_key : Locality) (user_key_addr : Addr)
+    (lkvs : kvs_logical_map) (m : kvs_user_map)
+    (E : coPset)
+    :
+
+    let fkey := (kvs_full_key user_key nkey) in
+
+    ↑(Nkvs.@"physical") ⊆ E ->
+
+    withinBounds user_key_addr (user_key_addr ^+ 1)%a user_key_addr = true ->
+    is_uint16 nkey ->
+
+    m !! nkey = None ->
+
+    ( na_inv cerise_nais (Nkvs.@"physical") kvs_inv ∗
+      na_own cerise_nais E ∗
+
+      (* initial register file *)
+      PC ↦ᵣ WCap RX Global KVS_pcc_b KVS_pcc_e kvs_addOrUpdate_pcc_addr ∗
+      cgp ↦ᵣ WCap RW Global KVS_cgp_b KVS_cgp_e KVS_cgp_b ∗
+      cra ↦ᵣ wret ∗
+      ca0 ↦ᵣ kvs_user_seal_key l_user_key user_key_addr ∗ (* Sealed User Key *)
+      ca1 ↦ᵣ WInt nkey ∗ (* Key to update *)
+      ca2 ↦ᵣ wca2 ∗ (* New value *)
+      ctp ↦ᵣ - ∗ (* scratch *)
+      ct1 ↦ᵣ - ∗ (* scratch *)
+      ct2 ↦ᵣ - ∗ (* scratch *)
+      cnull ↦ᵣ - ∗
+
+      (* initial memory layout *)
+      user_key_addr ↦ₐ WInt user_key ∗
+
+      ▷ ↪●LKVS lkvs ∗
+      ▷ is_logical_kvs lkvs ∗
+      ▷ user_key ↦(LKVS) m ∗
+
+      ▷ ( na_own cerise_nais E ∗
+          PC ↦ᵣ updatePcPerm wret ∗
+          cgp ↦ᵣ - ∗
+          cra ↦ᵣ - ∗
+          ca1 ↦ᵣ WInt 0 ∗
+          ca2 ↦ᵣ - ∗
+          ctp ↦ᵣ - ∗ (* scratch *)
+          ct1 ↦ᵣ - ∗ (* scratch *)
+          ct2 ↦ᵣ - ∗ (* scratch *)
+          cnull ↦ᵣ - ∗
+
+          user_key_addr ↦ₐ WInt user_key ∗
+
+          (
+            (* THERE IS AN EMPTY SLOT AVAILABLE*)
+            ( ⌜ canStore RW wca2 = true ⌝ ∗
+              ca0 ↦ᵣ WInt ASM_TRUE ∗ (* TRUE: an empty slot is available and is updated *)
+
+              ↪●LKVS (<<[ ( user_key, nkey ) := wca2 ]>> lkvs) ∗
+              is_logical_kvs (<<[ ( user_key, nkey ) := wca2 ]>> lkvs) ∗
+              user_key ↦(LKVS) (<[ nkey := wca2 ]> m)
+            )
+            ∨
+              (* THERE IS NO EMPTY SLOT AVAILABLE*)
+              (
+                ca0 ↦ᵣ WInt ASM_FALSE ∗ (* FALSE: no empty slot available *)
+                ↪●LKVS lkvs ∗
+                is_logical_kvs lkvs ∗
+                user_key ↦(LKVS) m
+              )
+          )
+          -∗
+          WP Seq (Instr Executable) {{ v, ⌜v = HaltedV⌝ → na_own cerise_nais ⊤ }}
+        )
+      ⊢ WP Seq (Instr Executable) {{ v, ⌜v = HaltedV⌝ → na_own cerise_nais ⊤ }})%I.
+  Proof.
+    intros fkey.
+    iIntros (Hnkvs_E Hbounds_a_user_key His_uint16_nkey Hm_nkey)
+      "( #Hkvs_inv & Hna
+        & HPC & Hcgp & Hcra & Hca0 & Hca1 & Hca2 & Hctp & Hct1 & Hct2 & Hcnull
+        & Ha_user_key
+        & >Hlkvs_auth & (%pkvs & >%Hsync & >Hpkvs_frag) & >Hm & Hpost)".
+    iMod (na_inv_acc with "Hkvs_inv Hna")
+      as "( (>Himports & >Hcode & (%pkvs' & HPKVS & >Hpkvs_frag')) & Hna & Hkvs_inv_close)"; eauto.
+
+    pose proof (HKVS_pcc_b' := KVS_size_imports).
+    pose proof (Hcode_continuous := KVS_size_code).
+    pose proof (Hcgp_continuous := KVS_size_data).
+    assert ((KVS_cgp_b + length kvs_data)%a = Some KVS_cgp_e) as Hbounds_cgp.
+    { by rewrite /length_kvs_data in Hcgp_continuous. }
+
+    rewrite /kvs_imports /kvs.kvs_imports_pre.
+    assert ((KVS_pcc_b + 1)%a = Some (KVS_pcc_b ^+ 1)%a) by ( rewrite /length_kvs_imports in HKVS_pcc_b'; solve_addr+ HKVS_pcc_b').
+    assert ((KVS_pcc_b ^+ 1)%a <= KVS_pcc_b')%a  by ( rewrite /length_kvs_imports in HKVS_pcc_b'; solve_addr+ HKVS_pcc_b').
+    assert ((KVS_pcc_b ^+ 1 + 1)%a = Some (KVS_pcc_b')%a) by ( rewrite /length_kvs_imports in HKVS_pcc_b'; solve_addr+ HKVS_pcc_b').
+    iDestruct (region_pointsto_cons with "Himports") as "[Himports_sw Himports]"; eauto.
+    iDestruct (region_pointsto_single with "Himports") as "(% & Ha_unsealing & %Heq)"; eauto; simplify_eq.
+    assert (SubBounds KVS_pcc_b KVS_pcc_e KVS_pcc_b' (KVS_pcc_b' ^+ length kvs_service_instrs)%a) as HSubBounds.
+    { solve_addr. }
+
+    focus_block_0 "Hcode" as "Hcode" "Hcont"; iHide "Hcont" as hcont.
+    assert (kvs_addOrUpdate_pcc_addr = KVS_pcc_b') as Heq_addr
+       by (rewrite /kvs_addOrUpdate_pcc_addr /kvs_addOrUpdate_pcc_off; solve_addr+HKVS_pcc_b').
+    rewrite -Heq_addr in H3; rewrite -Heq_addr.
+
+
+    iDestruct ( kvs_physical_kvs_valid with "Hpkvs_frag Hpkvs_frag'") as "<-".
+    iDestruct ( kvs_logical_kvs_valid with "Hlkvs_auth Hm" ) as "%Hlkvs_user_key".
+    pose proof (kvs_synced_logical_lookup_None _ _ _ _ _
+                  His_uint16_nkey Hsync Hlkvs_user_key Hm_nkey)
+      as Hpkvs_idx.
+
+
+    iApply (KVS_add_spec_layer_0 with
+             "[- $HPC $Hcgp $Hcra $Hca0 $Hca1 $Hca2 $Hctp $Hct1 $Hct2 $Hcnull
+              $Hcode $Ha_unsealing $Ha_user_key
+              $HPKVS]"); eauto.
+    iNext; iIntros "(HPC & Hcgp & Hcra & Hca1 & Hca2 & Hctp & Hct1 & Hct2 & Hcnull
+                     & Hcode & Ha_unsealing & Ha_user_key
+                     & [ (%idx_empty & %Hidx_empty & %Hcan_store & Hca0 & HPKVS)
+                         | (Hca0 & HPKVS)
+                       ] )".
+    all: rewrite Heq_addr; subst hcont; unfocus_block "Hcode" "Hcont" as "Hcode".
+    - iMod (kvs_physical_kvs_update (<[idx_empty:=Some (kvs_full_key user_key nkey, wca2)]> pkvs) with
+             "Hpkvs_frag Hpkvs_frag'") as "[Hpkvs_frag Hpkvs_frag']".
+      iMod ("Hkvs_inv_close" with "[$Hna $Hcode Himports_sw Ha_unsealing $HPKVS $Hpkvs_frag']") as "Hna" ; auto.
+      { iNext.
+        iApply (region_pointsto_cons with "[Ha_unsealing Himports_sw]"); eauto; iFrame.
+        iApply (region_pointsto_cons with "[Ha_unsealing]"); eauto; [solve_addr+|]; iFrame.
+        rewrite /region_pointsto finz_seq_between_empty; auto; solve_addr+.
+      }
+
+      iMod ( kvs_logical_kvs_update user_key _ _ (<[nkey := wca2]> m) with "Hlkvs_auth Hm" ) as "[Hlkvs_auth Hm]".
+      replace ( <[user_key:=<[nkey:=wca2]> m]> lkvs ) with ( <<[ (user_key, nkey):= wca2 ]>> lkvs ).
+      2: { rewrite /kvs_logical_kvs_insert Hlkvs_user_key //. }
+      eapply (kvs_synced_logical_kvs_insert _ _ _ _ _ wca2) in Hsync; eauto.
+
+
+      iApply "Hpost"; iFrame "∗%".
+      iLeft ; iFrame; done.
+
+    - iMod ("Hkvs_inv_close" with "[$Hna $Hcode Himports_sw Ha_unsealing $HPKVS $Hpkvs_frag']") as "Hna" ; auto.
+      { iNext.
+        iApply (region_pointsto_cons with "[Ha_unsealing Himports_sw]"); eauto; iFrame.
+        iApply (region_pointsto_cons with "[Ha_unsealing]"); eauto; [solve_addr+|]; iFrame.
+        rewrite /region_pointsto finz_seq_between_empty; auto; solve_addr+.
+      }
+
+      iApply "Hpost"; iFrame "∗%".
+      iRight ; iFrame.
+  Qed.
+
   Lemma KVS_add_spec_layer_2
     (wret wca2 : Word)
     (user_key : user_key_t) (nkey : map_key_t) (l_user_key : Locality) (user_key_addr : Addr)
@@ -580,14 +837,16 @@ Section KVS_spec_addOrUpdate.
     :
     let fkey := (kvs_full_key user_key nkey) in
 
-    ↑Nkvs ⊆ E ->
+    ↑(Nkvs.@"physical") ⊆ E ->
+    ↑(Nkvs.@"logical") ⊆ E ->
 
     is_uint16 nkey ->
     withinBounds user_key_addr (user_key_addr ^+ 1)%a user_key_addr = true ->
 
     m !! nkey = None ->
 
-    ( na_inv cerise_nais Nkvs kvs_inv ∗
+    ( na_inv cerise_nais (Nkvs.@"physical") kvs_inv ∗
+      na_inv cerise_nais (Nkvs.@"logical") logical_kvs_inv ∗
       na_own cerise_nais E ∗
 
       (* initial register file *)
@@ -636,42 +895,31 @@ Section KVS_spec_addOrUpdate.
       ⊢ WP Seq (Instr Executable) {{ v, ⌜v = HaltedV⌝ → na_own cerise_nais ⊤ }})%I.
   Proof.
     intros fkey.
-    iIntros (Hnkvs_E His_uint16_nkey Hbounds_a_user_key Hm_nkey)
-      "(#Hkvs_inv & Hna & HPC & Hcgp & Hcra & Hca0 & Hca1 & Hca2 & Hctp & Hct1 & Hct2 & Hcnull
+    iIntros (Hnkvs_E Hnkvs_E' His_uint16_nkey Hbounds_a_user_key Hm_nkey)
+      "(#Hkvs_inv & #Hkvs_logical_inv & Hna
+      & HPC & Hcgp & Hcra & Hca0 & Hca1 & Hca2 & Hctp & Hct1 & Hct2 & Hcnull
       & Ha_user_key & Hm & Hpost)".
-    iMod (na_inv_acc with "Hkvs_inv Hna")
-      as "( (>Himports & >Hcode & (%lkvs & Hlkvs_auth & HKVS) & Hspred) & Hna & Hkvs_inv_close)"; eauto.
-    pose proof (Hcgp_continuous := KVS_size_data).
-    pose proof (HKVS_pcc_b' := KVS_size_imports).
-    pose proof (Hcode_continuous := KVS_size_code).
-    assert (SubBounds KVS_pcc_b KVS_pcc_e KVS_pcc_b' (KVS_pcc_b' ^+ length kvs_service_instrs)%a) as HSubBounds.
-    { solve_addr. }
-    codefrag_facts "Hcode"; rename H into Hpc_contiguous.
-    rewrite /kvs_imports /kvs.kvs_imports_pre.
-    assert ((KVS_pcc_b + 1)%a = Some (KVS_pcc_b ^+ 1)%a) by ( rewrite /length_kvs_imports in HKVS_pcc_b'; solve_addr+ HKVS_pcc_b').
-    assert ((KVS_pcc_b ^+ 1)%a <= KVS_pcc_b')%a  by ( rewrite /length_kvs_imports in HKVS_pcc_b'; solve_addr+ HKVS_pcc_b').
-    assert ((KVS_pcc_b ^+ 1 + 1)%a = Some (KVS_pcc_b')%a) by ( rewrite /length_kvs_imports in HKVS_pcc_b'; solve_addr+ HKVS_pcc_b').
-    iDestruct (region_pointsto_cons with "Himports") as "[Himports_sw Himports]"; eauto.
-    iDestruct (region_pointsto_single with "Himports") as "(% & Ha_unsealing & %Heq)"; eauto; simplify_eq.
+    iMod (na_inv_acc with "Hkvs_logical_inv Hna")
+      as "( (%lkvs & Hlkvs_auth & HLKVS) & Hna & Hkvs_logical_inv_close)"; eauto.
 
-    rewrite /kvs_service_instrs.
-    focus_block_0 "Hcode" as "Hcode" "Hcont"; iHide "Hcont" as hcont.
-    assert (kvs_addOrUpdate_pcc_addr = KVS_pcc_b')
-      as -> by (rewrite /kvs_addOrUpdate_pcc_addr /kvs_addOrUpdate_pcc_off; solve_addr+HKVS_pcc_b').
-    iApply (KVS_add_spec_layer_1 with "[- $HPC]"); last iFrame "∗#%"; eauto.
-    iNext ; iIntros "(HPC & Hcgp & Hcra & Hca1 & Hca2 & Hctp & Hct1 & Hct2
-              & Hcnull & Hcode & Ha_unsealing & Ha_user_key
-              & [ (%Hcan_store & Hca0 & Hlkvs_auth & HKVS & Hm)
-                | (Hca0 & Hlkvs_auth & HKVS & Hm) ]
-              )".
-
-    all: subst hcont; unfocus_block "Hcode" "Hcont" as "Hcode".
-    all: iMod ("Hkvs_inv_close" with "[$Hna $Hcode Himports_sw Ha_unsealing $Hlkvs_auth $HKVS $Hspred]") as "Hna"
-    ; auto; last ( iApply "Hpost"; iFrame ; try (iLeft; iFrame; done) ; try (iRight; iFrame; done)).
-    all: iNext.
-    all: iApply (region_pointsto_cons with "[Ha_unsealing Himports_sw]"); eauto; iFrame.
-    all: iApply (region_pointsto_cons with "[Ha_unsealing]"); eauto; [solve_addr+|]; iFrame.
-    all: rewrite /region_pointsto finz_seq_between_empty; auto; solve_addr+.
+    iApply (KVS_add_spec_layer_1 with
+             "[- $Hkvs_inv
+                 $HPC $Hcgp $Hcra $Hca0 $Hca1 $Hca2 $Hctp $Hct1 $Hct2 $Hcnull
+                 $Ha_user_key
+                 $Hlkvs_auth $HLKVS $Hm]"); last iFrame; eauto.
+    {  solve_ndisj. }
+    iNext; iIntros "(Hna
+                     & HPC & Hcgp & Hcra & Hca1 & Hca2 & Hctp & Hct1 & Hct2 & Hcnull
+                     & Ha_user_key
+                     & [ (%Hcan_store & Hca0 & Hlkvs_auth & HLKVS & Hm)
+                     | (Hca0 & Hlkvs_auth & HLKVS & Hm)
+                     ])".
+    - iMod ("Hkvs_logical_inv_close" with "[$Hna $Hlkvs_auth $HLKVS]") as "Hna" ; auto.
+      iApply "Hpost"; iFrame "∗%".
+      iLeft ; iFrame; done.
+    - iMod ("Hkvs_logical_inv_close" with "[$Hna $Hlkvs_auth $HLKVS]") as "Hna" ; auto.
+      iApply "Hpost"; iFrame "∗%".
+      iRight ; iFrame; done.
   Qed.
 
   Lemma KVS_add_spec
@@ -681,12 +929,14 @@ Section KVS_spec_addOrUpdate.
     :
     let fkey := (kvs_full_key user_key nkey) in
 
-    ↑Nkvs ⊆ E ->
+    ↑(Nkvs.@"physical") ⊆ E ->
+    ↑(Nkvs.@"logical") ⊆ E ->
 
     is_uint16 nkey ->
     withinBounds user_key_addr (user_key_addr ^+ 1)%a user_key_addr = true ->
 
-    ( na_inv cerise_nais Nkvs kvs_inv ∗
+    ( na_inv cerise_nais (Nkvs.@"physical") kvs_inv ∗
+      na_inv cerise_nais (Nkvs.@"logical") logical_kvs_inv ∗
       na_own cerise_nais E ∗
 
       (* initial register file *)
@@ -703,7 +953,7 @@ Section KVS_spec_addOrUpdate.
 
       user_key_addr ↦ₐ WInt user_key ∗
 
-      ▷ logical_user_kvs_inv user_key ∗
+      ▷ user_kvs_inv user_key ∗
       ▷ (user_key, nkey) ↦(KVS) ⊥ ∗
 
       ▷ (na_own cerise_nais E ∗
@@ -717,7 +967,7 @@ Section KVS_spec_addOrUpdate.
          ct2 ↦ᵣ - ∗ (* scratch *)
          cnull ↦ᵣ - ∗
          user_key_addr ↦ₐ WInt user_key ∗
-         logical_user_kvs_inv user_key ∗
+         user_kvs_inv user_key ∗
          (
            (* THERE IS AN EMPTY SLOT AVAILABLE*)
            (
@@ -737,8 +987,9 @@ Section KVS_spec_addOrUpdate.
       ⊢ WP Seq (Instr Executable) {{ v, ⌜v = HaltedV⌝ → na_own cerise_nais ⊤ }})%I.
   Proof.
     intros fkey.
-    iIntros (Hnkvs_E His_uint16_nkey Hbounds_a_user_key)
-      "(#Hkvs_inv & Hna & HPC & Hcgp & Hcra & Hca0 & Hca1 & Hca2 & Hctp & Hct1 & Hct2 & Hcnull
+    iIntros (Hnkvs_E Hnkvs_E' His_uint16_nkey Hbounds_a_user_key)
+      "(#Hkvs_inv & #Hkvs_logical_inv & Hna
+      & HPC & Hcgp & Hcra & Hca0 & Hca1 & Hca2 & Hctp & Hct1 & Hct2 & Hcnull
       & Ha_user_key & (%ukvs & >Hukvs_auth & (%m & Hm & >%Hsync)) & >Hk & Hpost)".
 
     iDestruct (kvs_user_kvs_valid with "Hukvs_auth Hk") as "%Hk".
@@ -746,7 +997,7 @@ Section KVS_spec_addOrUpdate.
 
 
     iApply (KVS_add_spec_layer_2
-             with "[- $Hkvs_inv $Hna
+             with "[- $Hkvs_inv $Hkvs_logical_inv $Hna
                     $HPC $Hcgp $Hcra $Hca0 $Hca1 $Hca2 $Hctp $Hct1 $Hct2 $Hcnull
                     $Ha_user_key $Hm]"); eauto.
     iNext; iIntros "(Hna & HPC & Hcgp & Hcra & Hca1 & Hca2 & Hctp & Hct1 & Hct2 & Hcnull
@@ -755,10 +1006,10 @@ Section KVS_spec_addOrUpdate.
 
     - iMod ( kvs_user_kvs_update _ _ _ _ (Some wca2) with "Hukvs_auth Hk" ) as "[Hukvs_auth Hk]".
       apply (kvs_synced_logical_user_kvs_insert _ _ nkey wca2) in Hsync.
-      iAssert (logical_user_kvs_inv user_key)%I with "[$Hm $Hukvs_auth]" as "Hlukvs"; auto.
+      iAssert (user_kvs_inv user_key)%I with "[$Hm $Hukvs_auth]" as "Hlukvs"; auto.
       iApply "Hpost"; iFrame; iLeft; iFrame; done.
 
-    - iAssert (logical_user_kvs_inv user_key)%I with "[$Hm $Hukvs_auth]" as "Hlukvs"; auto.
+    - iAssert (user_kvs_inv user_key)%I with "[$Hm $Hukvs_auth]" as "Hlukvs"; auto.
       iApply "Hpost"; iFrame; iRight; iFrame; done.
   Qed.
 
@@ -834,11 +1085,11 @@ Section KVS_spec_addOrUpdate.
     (E : coPset)
     :
 
-    ↑Nkvs ⊆ E ->
+    ↑(Nkvs.@"physical") ⊆ E ->
 
     ¬ word_is_uint16 wca1 ->
 
-    ( na_inv cerise_nais Nkvs kvs_inv ∗
+    ( na_inv cerise_nais (Nkvs.@"physical") kvs_inv ∗
       na_own cerise_nais E ∗
 
       (* initial register file *)
@@ -863,7 +1114,7 @@ Section KVS_spec_addOrUpdate.
     iIntros (HE Hnkey_is_uint16)
       "(#Hkvs_inv & Hna & HPC & Hcra & Hca0 & Hca1 & Hct1 & Hcnull & Hpost)".
     iMod (na_inv_acc with "Hkvs_inv Hna")
-      as "( (>Himports & >Hcode & HKVS & Hspred) & Hna & Hkvs_inv_close)"; eauto.
+      as "( (>Himports & >Hcode & HKVS) & Hna & Hkvs_inv_close)"; eauto.
     pose proof (Hcgp_continuous := KVS_size_data).
     pose proof (HKVS_pcc_b' := KVS_size_imports).
     pose proof (Hcode_continuous := KVS_size_code).
@@ -880,7 +1131,7 @@ Section KVS_spec_addOrUpdate.
 
     subst hcont; unfocus_block "Hcode" "Hcont" as "Hcode".
 
-    iMod ("Hkvs_inv_close" with "[$Hna $Hcode $Himports $HKVS $Hspred]") as "Hna".
+    iMod ("Hkvs_inv_close" with "[$Hna $Hcode $Himports $HKVS]") as "Hna".
     iApply "Hpost"; iFrame.
   Qed.
 
@@ -953,12 +1204,12 @@ Section KVS_spec_addOrUpdate.
     (E : coPset)
     :
 
-    ↑Nkvs ⊆ E ->
+    ↑(Nkvs.@"physical") ⊆ E ->
 
     is_uint16 nkey ->
     is_sealed_with_o wca0 KVS_OTYPE = false ->
 
-    ( na_inv cerise_nais Nkvs kvs_inv ∗
+    ( na_inv cerise_nais (Nkvs.@"physical") kvs_inv ∗
       na_own cerise_nais E ∗
 
       (* initial register file *)
@@ -977,7 +1228,7 @@ Section KVS_spec_addOrUpdate.
     iIntros (HE Hnkey_is_uint16 Hwca0)
       "(#Hkvs_inv & Hna & HPC & Hcgp & Hcra & Hca0 & Hca1 & Hct1 & Hct2 & Hctp & Hcnull)".
     iMod (na_inv_acc with "Hkvs_inv Hna")
-      as "( (>Himports & >Hcode & HKVS & Hspred) & Hna & Hkvs_inv_close)"; eauto.
+      as "( (>Himports & >Hcode & HKVS) & Hna & Hkvs_inv_close)"; eauto.
     pose proof (Hcgp_continuous := KVS_size_data).
     pose proof (HKVS_pcc_b' := KVS_size_imports).
     pose proof (Hcode_continuous := KVS_size_code).
